\section{Derivation of Cases}

\subsection{Case 1}
  Conditions:
  \begin{IEEEeqnarray*}{rCl}
    RTT & < & T_{on} - \eta \\
    RTT & < & T_{off} - D - \tau
  \end{IEEEeqnarray*}
  Equations:
  \begin{IEEEeqnarray*}{rCl}
    Q & = & R_{on} RTT + \frac{\eta R_{on}}{2} \\
    R & = & C - R_{avg} \frac{2T_{on} + 2D + \tau - \eta}{2T_{on}}
  \end{IEEEeqnarray*}

\subsection{Case 2}
  Conditions:
  \begin{IEEEeqnarray*}{rCl}
    RTT & < & T_{on} \\
    RTT & \ge & T_{on} - \eta \\
    RTT & < & T_{on} + T_{off} - \eta \\
    RTT & < & T_{off} - D - \tau
  \end{IEEEeqnarray*}
  Equations:
  \begin{IEEEeqnarray*}{rCl}
    Q & = & R_{on} RTT + \frac{(R_{on} + R_{M2} - C + R_{on})(T_{on} - RTT)}
    {2} \\ 
    R & = & C - R_{avg} \frac{2T_{on} + 2D + \tau - \eta}{2T_{on}} \\
    R_{M2} & = & C + \frac{R_{on}(RTT - T_{on})}{\eta} \\
  \end{IEEEeqnarray*}

\subsection{Case 3}
  Conditions:
  \begin{IEEEeqnarray*}{rCl}
    RTT & \ge & T_{on} \\
    RTT & < & T_{on} + T_{off} - \eta \\
    RTT & < & T_{off} - D - \tau
  \end{IEEEeqnarray*}
  Equations:
  \begin{IEEEeqnarray*}{rCl}
    Q & = & R_{on}T_{on} \\
    R & = & C - R_{avg}\frac{2T_{on} + 2D + \tau - \eta}{2T_{on}}
  \end{IEEEeqnarray*}

\subsection{Case 4}
  Conditions:
  \begin{IEEEeqnarray*}{rCl}
    RTT & < & T_{on} - \eta \\
    RTT & < & T_{off} - D \\
    RTT & \ge & T_{on} - D - \tau \\
    RTT & < & T_{off} + T_{on} - D - \tau
  \end{IEEEeqnarray*}
  Equations:
  \begin{IEEEeqnarray*}{rCl}
    Q & = & \frac{(R_{on} + R_{M1} - C + R_{on})(RTT + D + \tau - T_{off})}{2}
    + R_{on}(T_{off} -D - \tau) + \frac{\eta R_{on}}{2} \\
    R & = & C - R_{avg}\frac{2T_{on} + 2D + \tau - \eta}{2T_{on}} \\
    R_{M1} & = & C + \frac{R_{on}(T_{off} - \tau - RTT - D)}{\tau}
  \end{IEEEeqnarray*}

\subsection{Case 5}
  Conditions:
  \begin{IEEEeqnarray*}{rCl}
    RTT & < & T_{on} \\
    RTT & \ge & T_{on} - \eta \\
    RTT & < & T_{on} + T_{off} - \eta \\
    RTT & < & T_{off} - D \\
    RTT & \ge & T_{off} - D - \tau \\
    RTT & < & T_{off} + T_{on} - D - \tau
  \end{IEEEeqnarray*}
  Equations:
  \begin{IEEEeqnarray*}{rCl}
    Q & = & \frac{(2R_{on} + R_{M1} - C)(RTT + D + \tau - T_{off})}
    {2} + R_{on}(T_{off} - D - \tau)  \\
    && + \frac{(2R_{on} + R_{M2} - C)(T_{on} - RTT)}{2} \\
    R & = & C - R_{avg}\frac{2T_{on} + 2D + \tau - \eta}{2T_{on}} \\
    R_{M1} & = & C + \frac{R_{on}(T_{off} - \tau - RTT - D)}{\tau} \\
    R_{M2} & = & C + \frac{R_{on}(RTT - T_{on})}{\eta}
  \end{IEEEeqnarray*}

\subsection{Case 6}
  Conditions:
  \begin{IEEEeqnarray*}{rCl}
    RTT & \ge & T_{on} \\
    RTT & < & T_{on} + T_{off} - \eta \\
    RTT & < & T_{off} - D \\
    RTT & \ge & T_{off} - D - \tau \\
    RTT & < & T_{off} + T_{on} - D - \tau
  \end{IEEEeqnarray*}
  Equations:
  \begin{IEEEeqnarray*}{rCl}
    Q & = & \frac{(2R_{on} + R_{M1} - C)(RTT + D + \tau - T_{off})}{2} + 
    R_{on}(T_{off} + T_{on} - RTT - D - \tau) \\
    R & = & C - R_{avg}\frac{2T_{on} + 2D + \tau - \eta}{2T_{on}} \\
    R_{M1} & = & C + \frac{R_{on}(T_{off} - \tau - RTT - D)}{\tau}
  \end{IEEEeqnarray*}

\subsection{Case 7}
  Conditions:
  \begin{IEEEeqnarray*}{rCl}
    RTT & < & T_{on} - \eta \\
    RTT & \ge & T_{off} - D \\
    RTT & < & T_{off} + T_{on} - D - \tau
  \end{IEEEeqnarray*}
  Equations:
  \begin{IEEEeqnarray*}{rCl}
    Q & = & \frac{\tau R_{on}}{2} + R_{on}(T_{off} - D - \tau) + \frac{\eta 
    R_{on}}{2} \\
    R & = & C - R_{avg}\frac{2T_{on} + 2D + \tau - \eta}{2T_{on}}
  \end{IEEEeqnarray*}

\subsection{Case 8}
  Conditions:
  \begin{IEEEeqnarray*}{rCl}
    RTT & < & T_{on} \\
    RTT & \ge & T_{on} - \eta \\
    RTT & < & T_{on} + T_{off} - \eta \\
    RTT & \ge & T_{off} - D \\
    RTT & < & T_{off} + T_{on} - D - \tau
  \end{IEEEeqnarray*}
  Equations:
  \begin{IEEEeqnarray*}{rCl}
    Q & = & \frac{\tau R_{on}}{2} + R_{on}(T_{off} - D - \tau) +
    \frac{(2R_{on} + R_{M2} - C)(T_{on} - RTT)}{2} \\
    R & = & C - R_{avg}\frac{2T_{on} + 2D + \tau - \eta}{2T_{on}} \\
    R_{M2} & = & C + \frac{R_{on} (RTT - T_{on})}{\eta}
  \end{IEEEeqnarray*}

\subsection{Case 9}
  Conditions:
  \begin{IEEEeqnarray*}{rCl}
    RTT & \ge & T_{on} \\
    RTT & < & T_{on} + T_{off} - \eta \\
    RTT & \ge & T_{off} - D \\
    RTT & < & T_{off} + T_{on} - D - \tau
  \end{IEEEeqnarray*}
  Equations:
  \begin{IEEEeqnarray*}{rCl}
    Q & = & \frac{\tau R_{on}}{2} + R_{on}(T_{off} + T_{on} - RTT - D - \tau)\\
    R & = & C - R_{avg}\frac{2T_{on} + 2D + \tau - \eta}{2T_{on}}
  \end{IEEEeqnarray*}

\subsection{Case 10}
  Conditions:
  \begin{IEEEeqnarray*}{rCl}
    RTT & \ge & T_{on} \\
    RTT & < & T_{on} + T_{off} - \eta \\
    RTT & \ge & T_{off} - D \\
    RTT & < & T_{off} + T_{on} - D \\
    RTT & \ge & T_{off} + T_{on} - D - \tau \\
    RTT & < & 2T_{off} + T_{on} - D - \tau
  \end{IEEEeqnarray*}
  Equations:
  \begin{IEEEeqnarray*}{rCl}
    Q & = & \frac{(T_{off} + T_{on} - RTT - D)(R_{M2} - C + R_{on})}{2} \\
    R & = & C - R_{avg}\frac{2T_{on} + 2D + \tau - \eta}{2T_{on}} \\
    R_{M2} & = & C + \frac{R_{on}(T_{off} + T_{on} - \tau - RTT - D)}{\tau}
  \end{IEEEeqnarray*}

\subsection{Case 11}
  Conditions:
  \begin{IEEEeqnarray*}{rCl}
    RTT & \ge & T_{on} \\
    RTT & < & T_{on} + T_{off} \\
    RTT & \ge & T_{on} + T_{off} - \eta \\
    RTT & < & 2T_{on} + T_{off} - \eta \\
    RTT & \ge & T_{off} - D \\
    RTT & < & T_{off} + T_{on} - D - \tau
  \end{IEEEeqnarray*}
  Equations:
  \begin{IEEEeqnarray*}{rCl}
    Q & = & \frac{(RTT + \eta - T_{on} - T_{off})(R_{M1} - C + R_{on})}{2} + 
    \frac{\tau R_{on}}{2} + R_{on} (T_{off} + T_{on} - RTT - D - \tau) \\
    R & = & C - R_{avg}\frac{2T_{on} + 2D + \tau - \eta}{2T_{on}} \\
    R_{M1} & = & C + \frac{R_{on}(RTT - T_{off} - T_{on})}{\eta}
  \end{IEEEeqnarray*}

\subsection{Case 12}
  Conditions:
  \begin{IEEEeqnarray*}{rCl}
    RTT & \ge & T_{on} \\
    RTT & < & T_{on} + T_{off} \\
    RTT & \ge & T_{on} + T_{off} - \eta \\
    RTT & < & 2T_{on} + T_{off} - \eta \\
    RTT & \ge & T_{off} - D \\
    RTT & < & T_{off} + T_{on} - D \\
    RTT & \ge & T_{off} + T_{on} - D - \tau \\
    RTT & < & 2T_{off} + T_{on} - D - \tau
  \end{IEEEeqnarray*}
  Equations:
  \begin{IEEEeqnarray*}{rCl}
    Q & = & \frac{(RTT + \eta - T_{on} - T_{off})(R_{M1} - C + R_{on})}{2} + 
    \frac{(T_{off} + T_{on} - RTT - D)(R_{M2} - C + R_{on})}{2} \\
    R & = & C - R_{avg}\frac{2T_{on} + 2D + \tau - \eta}{2T_{on}} \\
    R_{M1} & = & C + \frac{R_{on} (RTT - T_{off} - T_{on})}{\eta} \\
    R_{M2} & = & C + \frac{R_{on} (T_{off} + T_{on} - \tau - RTT - D)}{\tau}
  \end{IEEEeqnarray*}

\subsection{Case 13}
  Conditions:
  \begin{IEEEeqnarray*}{rCl}
    RTT & \ge & T_{on} \\
    RTT & < & T_{on} + T_{off} \\
    RTT & \ge & T_{on} + T_{off} - \eta \\
    RTT & < & 2T_{on} + T_{off} - \eta \\
    RTT & \ge & T_{off} + T_{on} - D \\
    RTT & < & 2T_{off} + T_{on} - D - \tau
  \end{IEEEeqnarray*}
  Equations:
  \begin{IEEEeqnarray*}{rCl}
    Q & = & \frac{(RTT + \eta - T_{on} - T_{off})(R_{M1} - C + R_{on})}{2} \\
    R & = & C - R_{avg}\frac{2T_{on} + 2D + \tau - \eta}{2T_{on}} \\
    R_{M1} & = & C + \frac{R_{on}(RTT - T_{off} - T_{on})}{\eta}
  \end{IEEEeqnarray*}

\subsection{Case 14}
  Conditions:
  \begin{IEEEeqnarray*}{rCl}
    RTT & < & T_{on} \\
    RTT & \ge & T_{on} + T_{off} - \eta \\
    RTT & < & 2T_{on} + T_{off} - \eta \\
    RTT & \ge & T_{off} - D \\
    RTT & < & T_{off} + T_{on} - D - \tau
  \end{IEEEeqnarray*}
  Equations:
  \begin{IEEEeqnarray*}{rCl}
    Q & = & \frac{(RTT + \eta - T_{on} - T_{off})(R_{M1} - C + R_{on})}{2} + 
    \frac{\tau R_{on}}{2} + R_{on}(T_{off} - D - \tau) \\ 
    && + \frac{(2R_{on} + R_{M2} - C)(T_{on} - RTT)}{2} \\
    R & = & C - R_{avg}\frac{2T_{on} + 2D + \tau - \eta}{2T_{on}} \\
    R_{M1} & = & C + \frac{R_{on}(RTT - T_{off} - T_{on})}{\eta} \\
    R_{M2} & = & C + \frac{R_{on}(RTT - T_{on})}{\eta}
  \end{IEEEeqnarray*}

\subsection{Case 15}
  Conditions:
  \begin{IEEEeqnarray*}{rCl}
    RTT & \ge & T_{on} \\
    RTT & < & T_{on} + T_{off} + \eta \\
    RTT & < & T_{off} - D \\
    RTT & \ge & T_{off} + T_{on} - D - \tau \\
    RTT & < & 2T_{off} + T_{on} - D - \tau
  \end{IEEEeqnarray*}
  Equations:
  \begin{IEEEeqnarray*}{rCl}
    Q & = & \frac{(R_{M1} + R_{M2} - 2C + 2R_{on})T_{on}}{2} \\
    R & = & C - R_{avg}\frac{2T_{on} + 2D + \tau - \eta}{2T_{on}} \\
    R_{M1} & = & C + \frac{R_{on}(T_{off} - \tau - D - RTT)}{\tau} \\
    R_{M2} & = & C + \frac{R_{on}(T_{off} + T_{on} - \tau - D - RTT)}{\tau}
  \end{IEEEeqnarray*}

\subsection{Case 16}
  Conditions:
  \begin{IEEEeqnarray*}{rCl}
    RTT & \ge & T_{on} \\
    RTT & < & T_{on} + T_{off} \\
    RTT & \ge & 2T_{on} + T_{off} - \eta \\
    RTT & < & 2T_{on} + 2T_{off} - \eta \\
    RTT & \ge & T_{off} + T_{on} - D \\
    RTT & < & 2T_{off} + T_{on} - D - \tau
  \end{IEEEeqnarray*}
  Equations:
  \begin{IEEEeqnarray*}{rCl}
    Q & = & \frac{(R_{M1} + R_{M2} - 2C + 2R_{on})T_{on}}{2} \\
    R & = & C - R_{avg}\frac{2T_{on} + 2D + \tau - \eta}{2T_{on}} \\
    R_{M1} & = & C + \frac{R_{on}(RTT - T_{off} - T_{on})}{\eta} \\
    R_{M2} & = & C + \frac{R_{on}(RTT - T_{off} - 2T_{on})}{\eta}
  \end{IEEEeqnarray*}

\subsection{Case 17}
  Conditions:
  \begin{IEEEeqnarray*}{rCl}
    RTT & < & T_{on} \\
    RTT & < & T_{off} - D \\
    RTT & \ge & T_{off} - D - \tau \\
    RTT & < & T_{off} + T_{on} - D - \tau
  \end{IEEEeqnarray*}
  Equations:
  \begin{IEEEeqnarray*}{rCl}
    Q & = & \frac{R_{M1} - C + 2R_{on})(RTT + D + \tau - T_{off})}{2} +
    R_{on}(T_{off} - D - \tau) \\ 
    && + \frac{(R_{on} + R_{M2} - C + R_{on})*T_{on} - RTT)}{2} \\
    R & = & \left (\frac{C + R_L}{2} \right ) \left (\frac{T_{on} + D + \tau}
    {T_{on} + T_{off}} \right ) + C \left (\frac{T_{off} - D - \tau}
    {T_{on} + T_{off}} \right ) \\
    R_{M1} & = & \frac{D R_L - C RTT + R_L RTT + C T_{off} - R_L T_{off} 
    R_L \tau - C D}{\tau} \\
    R_{M2} & = & C + \frac{R_{on}(RTT -T_{on})}{\eta} \\
    R_L & = & C - \frac{R_{on}(T_{on} + D)}{\eta}
  \end{IEEEeqnarray*}

\subsection{Case 18}
  Conditions:
  \begin{IEEEeqnarray*}{rCl}
    RTT & < & T_{on} \\
    RTT & \ge & T_{off} - D \\
    RTT & < & T_{on} + T_{off} - D \\
    RTT & < & T_{off} + T_{on} - D - \tau
  \end{IEEEeqnarray*}
  Equations:
  \begin{IEEEeqnarray*}{rCl}
    Q & = & \frac{(R_{M1} -2C + 2R_{on} + R_L)(RTT + D - T_{off})}{2} + 
    \frac{(R_L - C + 2R_{on})\tau}{2} \\ 
    && + R_{on}(T_{off} - D - \tau) + 
    \frac{(2R_{on} + R_{M2} - C)(T_{on} - RTT)}{2} \\ 
    R & = & \left (\frac{C + R_L}{2} \right ) \left (\frac{T_{on} + D + \tau}
    {T_{on} + T_{off}} \right ) + C \left (\frac{T_{off} - D - \tau}
    {T_{on} + T_{off}} \right ) \\
    R_{M1} & = & C + \frac{R_{on}(RTT - T_{off} - T_{on})}{\eta} \\
    R_{M2} & = & C + \frac{R_{on} (RTT - T_{on})}{\eta} \\
    R_L & = & C - \frac{R_{on}(T_{on} + D)}{\eta}
  \end{IEEEeqnarray*}

\subsection{Case 19}
  Conditions:
  \begin{IEEEeqnarray*}{rCl}
    RTT & \ge & T_{on} \\
    RTT & < & T_{off} - D \\
    RTT & < & T_{off} - D - \tau
  \end{IEEEeqnarray*}
  Equations:
  \begin{IEEEeqnarray*}{rCl}
    Q & = & R_{on} T_{on} \\
    R & = & \left (\frac{C + R_L}{2} \right ) \left (\frac{T_{on} + D + \tau}
    {T_{on} + T_{off}} \right ) + C \left (\frac{T_{off} - D - \tau}
    {T_{on} + T_{off}} \right ) \\
    R_L & = & C - \frac{R_{on}(T_{on} + D)}{\eta}
  \end{IEEEeqnarray*}

\subsection{Case 20}
  Conditions:
  \begin{IEEEeqnarray*}{rCl}
    RTT & \ge & T_{on} \\
    RTT & < & T_{on} + T_{off} \\
    RTT & \ge & T_{off} - D \\
    RTT & < & T_{off} + T_{on} - D - \tau
  \end{IEEEeqnarray*}
  Equations:
  \begin{IEEEeqnarray*}{rCl}
    Q & = & \frac{(R_{M1} - 2C + R_L + 2R_{on})(RTT + D - T_{off})}{2} +
    \frac{(R_L - C + 2R_{on})\tau}{2} \\
    && + R_{on}(T_{off} + T_{on} - RTT - D - \tau) \\
    R & = & \left (\frac{C + R_L}{2} \right ) \left (\frac{T_{on} + D + \tau}
    {T_{on} + T_{off}} \right ) + C \left (\frac{T_{off} - D - \tau}
    {T_{on} + T_{off}} \right ) \\
    R_{M1} & = & C + \frac{R_{on}(RTT - T_{off} - T_{on})}{\eta} \\
    R_L & = & C - \frac{R_{on}(T_{on} + D)}{\eta}
  \end{IEEEeqnarray*}

\subsection{Case 21}
  Conditions:
  \begin{IEEEeqnarray*}{rCl}
    RTT & < & T_{on} - \eta \\
    RTT & < & T_{off} - D - \tau
  \end{IEEEeqnarray*}
  Equations:
  \begin{IEEEeqnarray*}{rCl}
    Q & = & R_{on} RTT + \frac{\eta R_{on}}{2} \\
    R & = & C - R_{avg} \frac{2T_{on} + 2D + \tau - \eta}{2T_{on}}
  \end{IEEEeqnarray*}

\subsection{Case 22}
  Conditions:
  \begin{IEEEeqnarray*}{rCl}
    RTT & < & T_{on} \\
    RTT & \ge & T_{on} - \eta \\
    RTT & < & T_{on} + T_{off} - \eta \\
    RTT & < & T_{off} - D - \tau
  \end{IEEEeqnarray*}
  Equations:
  \begin{IEEEeqnarray*}{rCl}
    Q & = & R_{on} RTT + \frac{(R_{on} + R_{M2} - C + R_{on})(T_{on} - RTT)}
    {2} \\ 
    R & = & C - R_{avg} \frac{2T_{on} + 2D + \tau - \eta}{2T_{on}} \\
    R_{M2} & = & C + \frac{R_{on}(RTT - T_{on})}{\eta} \\
  \end{IEEEeqnarray*}

\subsection{Case 23}
  Conditions:
  \begin{IEEEeqnarray*}{rCl}
    RTT & \ge & T_{on} \\
    RTT & < & T_{on} + T_{off} - \eta \\
    RTT & < & T_{off} - D - \tau
  \end{IEEEeqnarray*}
  Equations:
  \begin{IEEEeqnarray*}{rCl}
    Q & = & R_{on}T_{on} \\
    R & = & C - R_{avg}\frac{2T_{on} + 2D + \tau - \eta}{2T_{on}}
  \end{IEEEeqnarray*}

\subsection{Case 24}
  Conditions:
  \begin{IEEEeqnarray*}{rCl}
    RTT & < & T_{on} - \eta \\
    RTT & < & T_{off} - D \\
    RTT & \ge & T_{on} - D - \tau \\
    RTT & < & T_{off} + T_{on} - D - \tau
  \end{IEEEeqnarray*}
  Equations:
  \begin{IEEEeqnarray*}{rCl}
    Q & = & \frac{(R_{on} + R_{M1} - C + R_{on})(RTT + D + \tau - T_{off})}{2}
    + R_{on}(T_{off} -D - \tau) + \frac{\eta R_{on}}{2} \\
    R & = & C - R_{avg}\frac{2T_{on} + 2D + \tau - \eta}{2T_{on}} \\
    R_{M1} & = & C + \frac{R_{on}(T_{off} - \tau - RTT - D)}{\tau}
  \end{IEEEeqnarray*}

\subsection{Case 25}
  Conditions:
  \begin{IEEEeqnarray*}{rCl}
    RTT & < & T_{on} \\
    RTT & \ge & T_{on} - \eta \\
    RTT & < & T_{on} + T_{off} - \eta \\
    RTT & < & T_{off} - D \\
    RTT & \ge & T_{off} - D - \tau \\
    RTT & < & T_{off} + T_{on} - D - \tau
  \end{IEEEeqnarray*}
  Equations:
  \begin{IEEEeqnarray*}{rCl}
    Q & = & \frac{(2R_{on} + R_{M1} - C)(RTT + D + \tau - T_{off})}
    {2} + R_{on}(T_{off} - D - \tau)  \\
    && + \frac{(2R_{on} + R_{M2} - C)(T_{on} - RTT)}{2} \\
    R & = & C - R_{avg}\frac{2T_{on} + 2D + \tau - \eta}{2T_{on}} \\
    R_{M1} & = & C + \frac{R_{on}(T_{off} - \tau - RTT - D)}{\tau} \\
    R_{M2} & = & C + \frac{R_{on}(RTT - T_{on})}{\eta}
  \end{IEEEeqnarray*}

\subsection{Case 26}
  Conditions:
  \begin{IEEEeqnarray*}{rCl}
    RTT & \ge & T_{on} \\
    RTT & < & T_{on} + T_{off} - \eta \\
    RTT & < & T_{off} - D \\
    RTT & \ge & T_{off} - D - \tau \\
    RTT & < & T_{off} + T_{on} - D - \tau
  \end{IEEEeqnarray*}
  Equations:
  \begin{IEEEeqnarray*}{rCl}
    Q & = & \frac{(2R_{on} + R_{M1} - C)(RTT + D + \tau - T_{off})}{2} + 
    R_{on}(T_{off} + T_{on} - RTT - D - \tau) \\
    R & = & C - R_{avg}\frac{2T_{on} + 2D + \tau - \eta}{2T_{on}} \\
    R_{M1} & = & C + \frac{R_{on}(T_{off} - \tau - RTT - D)}{\tau}
  \end{IEEEeqnarray*}

\subsection{Case 27}
  Conditions:
  \begin{IEEEeqnarray*}{rCl}
    RTT & < & T_{on} - \eta \\
    RTT & \ge & T_{off} - D \\
    RTT & < & T_{off} + T_{on} - D - \tau
  \end{IEEEeqnarray*}
  Equations:
  \begin{IEEEeqnarray*}{rCl}
    Q & = & \frac{\tau R_{on}}{2} + R_{on}(T_{off} - D - \tau) + \frac{\eta 
    R_{on}}{2} \\
    R & = & C - R_{avg}\frac{2T_{on} + 2D + \tau - \eta}{2T_{on}}
  \end{IEEEeqnarray*}

\subsection{Case 28}
  Conditions:
  \begin{IEEEeqnarray*}{rCl}
    RTT & < & T_{on} \\
    RTT & \ge & T_{on} - \eta \\
    RTT & < & T_{on} + T_{off} - \eta \\
    RTT & \ge & T_{off} - D \\
    RTT & < & T_{off} + T_{on} - D - \tau
  \end{IEEEeqnarray*}
  Equations:
  \begin{IEEEeqnarray*}{rCl}
    Q & = & \frac{\tau R_{on}}{2} + R_{on}(T_{off} - D - \tau) +
    \frac{(2R_{on} + R_{M2} - C)(T_{on} - RTT)}{2} \\
    R & = & C - R_{avg}\frac{2T_{on} + 2D + \tau - \eta}{2T_{on}} \\
    R_{M2} & = & C + \frac{R_{on} (RTT - T_{on})}{\eta}
  \end{IEEEeqnarray*}

\subsection{Case 29}
  Conditions:
  \begin{IEEEeqnarray*}{rCl}
    RTT & \ge & T_{on} \\
    RTT & < & T_{on} + T_{off} - \eta \\
    RTT & \ge & T_{off} - D \\
    RTT & < & T_{off} + T_{on} - D - \tau
  \end{IEEEeqnarray*}
  Equations:
  \begin{IEEEeqnarray*}{rCl}
    Q & = & \frac{\tau R_{on}}{2} + R_{on}(T_{off} + T_{on} - RTT - D - \tau)\\
    R & = & C - R_{avg}\frac{2T_{on} + 2D + \tau - \eta}{2T_{on}}
  \end{IEEEeqnarray*}

\subsection{Case 30}
  Conditions:
  \begin{IEEEeqnarray*}{rCl}
    RTT & \ge & T_{on} \\
    RTT & < & T_{on} + T_{off} - \eta \\
    RTT & \ge & T_{off} - D \\
    RTT & < & T_{off} + T_{on} - D \\
    RTT & \ge & T_{off} + T_{on} - D - \tau \\
    RTT & < & 2T_{off} + T_{on} - D - \tau
  \end{IEEEeqnarray*}
  Equations:
  \begin{IEEEeqnarray*}{rCl}
    Q & = & \frac{(T_{off} + T_{on} - RTT - D)(R_{M2} - C + R_{on})}{2} \\
    R & = & C - R_{avg}\frac{2T_{on} + 2D + \tau - \eta}{2T_{on}} \\
    R_{M2} & = & C + \frac{R_{on}(T_{off} + T_{on} - \tau - RTT - D)}{\tau}
  \end{IEEEeqnarray*}

\subsection{Case 31}
  Conditions:
  \begin{IEEEeqnarray*}{rCl}
    RTT & \ge & T_{on} \\
    RTT & < & T_{on} + T_{off} \\
    RTT & \ge & T_{on} + T_{off} - \eta \\
    RTT & < & 2T_{on} + T_{off} - \eta \\
    RTT & \ge & T_{off} - D \\
    RTT & < & T_{off} + T_{on} - D - \tau
  \end{IEEEeqnarray*}
  Equations:
  \begin{IEEEeqnarray*}{rCl}
    Q & = & \frac{(RTT + \eta - T_{on} - T_{off})(R_{M1} - C + R_{on})}{2} + 
    \frac{\tau R_{on}}{2} + R_{on} (T_{off} + T_{on} - RTT - D - \tau) \\
    R & = & C - R_{avg}\frac{2T_{on} + 2D + \tau - \eta}{2T_{on}} \\
    R_{M1} & = & C + \frac{R_{on}(RTT - T_{off} - T_{on})}{\eta}
  \end{IEEEeqnarray*}

\subsection{Case 32}
  Conditions:
  \begin{IEEEeqnarray*}{rCl}
    RTT & \ge & T_{on} \\
    RTT & < & T_{on} + T_{off} \\
    RTT & \ge & T_{on} + T_{off} - \eta \\
    RTT & < & 2T_{on} + T_{off} - \eta \\
    RTT & \ge & T_{off} - D \\
    RTT & < & T_{off} + T_{on} - D \\
    RTT & \ge & T_{off} + T_{on} - D - \tau \\
    RTT & < & 2T_{off} + T_{on} - D - \tau
  \end{IEEEeqnarray*}
  Equations:
  \begin{IEEEeqnarray*}{rCl}
    Q & = & \frac{(RTT + \eta - T_{on} - T_{off})(R_{M1} - C + R_{on})}{2} + 
    \frac{(T_{off} + T_{on} - RTT - D)(R_{M2} - C + R_{on})}{2} \\
    R & = & C - R_{avg}\frac{2T_{on} + 2D + \tau - \eta}{2T_{on}} \\
    R_{M1} & = & C + \frac{R_{on} (RTT - T_{off} - T_{on})}{\eta} \\
    R_{M2} & = & C + \frac{R_{on} (T_{off} + T_{on} - \tau - RTT - D)}{\tau}
  \end{IEEEeqnarray*}

\subsection{Case 33}
  Conditions:
  \begin{IEEEeqnarray*}{rCl}
    RTT & \ge & T_{on} \\
    RTT & < & T_{on} + T_{off} \\
    RTT & \ge & T_{on} + T_{off} - \eta \\
    RTT & < & 2T_{on} + T_{off} - \eta \\
    RTT & \ge & T_{off} + T_{on} - D \\
    RTT & < & 2T_{off} + T_{on} - D - \tau
  \end{IEEEeqnarray*}
  Equations:
  \begin{IEEEeqnarray*}{rCl}
    Q & = & \frac{(RTT + \eta - T_{on} - T_{off})(R_{M1} - C + R_{on})}{2} \\
    R & = & C - R_{avg}\frac{2T_{on} + 2D + \tau - \eta}{2T_{on}} \\
    R_{M1} & = & C + \frac{R_{on}(RTT - T_{off} - T_{on})}{\eta}
  \end{IEEEeqnarray*}

\subsection{Case 34}
  Conditions:
  \begin{IEEEeqnarray*}{rCl}
    RTT & < & T_{on} \\
    RTT & \ge & T_{on} + T_{off} - \eta \\
    RTT & < & 2T_{on} + T_{off} - \eta \\
    RTT & \ge & T_{off} - D \\
    RTT & < & T_{off} + T_{on} - D - \tau
  \end{IEEEeqnarray*}
  Equations:
  \begin{IEEEeqnarray*}{rCl}
    Q & = & \frac{(RTT + \eta - T_{on} - T_{off})(R_{M1} - C + R_{on})}{2} + 
    \frac{\tau R_{on}}{2} + R_{on}(T_{off} - D - \tau) \\ 
    && + \frac{(2R_{on} + R_{M2} - C)(T_{on} - RTT)}{2} \\
    R & = & C - R_{avg}\frac{2T_{on} + 2D + \tau - \eta}{2T_{on}} \\
    R_{M1} & = & C + \frac{R_{on}(RTT - T_{off} - T_{on})}{\eta} \\
    R_{M2} & = & C + \frac{R_{on}(RTT - T_{on})}{\eta}
  \end{IEEEeqnarray*}

\subsection{Case 35}
  Conditions:
  \begin{IEEEeqnarray*}{rCl}
    RTT & \ge & T_{on} \\
    RTT & < & T_{on} + T_{off} + \eta \\
    RTT & < & T_{off} - D \\
    RTT & \ge & T_{off} + T_{on} - D - \tau \\
    RTT & < & 2T_{off} + T_{on} - D - \tau
  \end{IEEEeqnarray*}
  Equations:
  \begin{IEEEeqnarray*}{rCl}
    Q & = & \frac{(R_{M1} + R_{M2} - 2C + 2R_{on})T_{on}}{2} \\
    R & = & C - R_{avg}\frac{2T_{on} + 2D + \tau - \eta}{2T_{on}} \\
    R_{M1} & = & C + \frac{R_{on}(T_{off} - \tau - D - RTT)}{\tau} \\
    R_{M2} & = & C + \frac{R_{on}(T_{off} + T_{on} - \tau - D - RTT)}{\tau}
  \end{IEEEeqnarray*}

\subsection{Case 36}
  Conditions:
  \begin{IEEEeqnarray*}{rCl}
    RTT & \ge & T_{on} \\
    RTT & < & T_{on} + T_{off} \\
    RTT & \ge & 2T_{on} + T_{off} - \eta \\
    RTT & < & 2T_{on} + 2T_{off} - \eta \\
    RTT & \ge & T_{off} + T_{on} - D \\
    RTT & < & 2T_{off} + T_{on} - D - \tau
  \end{IEEEeqnarray*}
  Equations:
  \begin{IEEEeqnarray*}{rCl}
    Q & = & \frac{(R_{M1} + R_{M2} - 2C + 2R_{on})T_{on}}{2} \\
    R & = & C - R_{avg}\frac{2T_{on} + 2D + \tau - \eta}{2T_{on}} \\
    R_{M1} & = & C + \frac{R_{on}(RTT - T_{off} - T_{on})}{\eta} \\
    R_{M2} & = & C + \frac{R_{on}(RTT - T_{off} - 2T_{on})}{\eta}
  \end{IEEEeqnarray*}

\subsection{Case 37}
  Conditions:
  \begin{IEEEeqnarray*}{rCl}
    RTT & < & T_{on} \\
    RTT & < & T_{off} - D \\
    RTT & \ge & T_{off} - D - \tau \\
    RTT & < & T_{off} + T_{on} - D - \tau
  \end{IEEEeqnarray*}
  Equations:
  \begin{IEEEeqnarray*}{rCl}
    Q & = & \frac{R_{M1} - C + 2R_{on})(RTT + D + \tau - T_{off})}{2} +
    R_{on}(T_{off} - D - \tau) \\ 
    && + \frac{(R_{on} + R_{M2} - C + R_{on})*T_{on} - RTT)}{2} \\
    R & = & \left (\frac{C + R_L}{2} \right ) \left (\frac{T_{on} + D + \tau}
    {T_{on} + T_{off}} \right ) + C \left (\frac{T_{off} - D - \tau}
    {T_{on} + T_{off}} \right ) \\
    R_{M1} & = & \frac{D R_L - C RTT + R_L RTT + C T_{off} - R_L T_{off} 
    R_L \tau - C D}{\tau} \\
    R_{M2} & = & C + \frac{R_{on}(RTT -T_{on})}{\eta} \\
    R_L & = & C - \frac{R_{on}(T_{on} + D)}{\eta}
  \end{IEEEeqnarray*}

\subsection{Case 38}
  Conditions:
  \begin{IEEEeqnarray*}{rCl}
    RTT & < & T_{on} \\
    RTT & \ge & T_{off} - D \\
    RTT & < & T_{on} + T_{off} - D \\
    RTT & < & T_{off} + T_{on} - D - \tau
  \end{IEEEeqnarray*}
  Equations:
  \begin{IEEEeqnarray*}{rCl}
    Q & = & \frac{(R_{M1} -2C + 2R_{on} + R_L)(RTT + D - T_{off})}{2} + 
    \frac{(R_L - C + 2R_{on})\tau}{2} \\ 
    && + R_{on}(T_{off} - D - \tau) + 
    \frac{(2R_{on} + R_{M2} - C)(T_{on} - RTT)}{2} \\ 
    R & = & \left (\frac{C + R_L}{2} \right ) \left (\frac{T_{on} + D + \tau}
    {T_{on} + T_{off}} \right ) + C \left (\frac{T_{off} - D - \tau}
    {T_{on} + T_{off}} \right ) \\
    R_{M1} & = & C + \frac{R_{on}(RTT - T_{off} - T_{on})}{\eta} \\
    R_{M2} & = & C + \frac{R_{on} (RTT - T_{on})}{\eta} \\
    R_L & = & C - \frac{R_{on}(T_{on} + D)}{\eta}
  \end{IEEEeqnarray*}

\subsection{Case 39}
  Conditions:
  \begin{IEEEeqnarray*}{rCl}
    RTT & \ge & T_{on} \\
    RTT & < & T_{off} - D \\
    RTT & < & T_{off} - D - \tau
  \end{IEEEeqnarray*}
  Equations:
  \begin{IEEEeqnarray*}{rCl}
    Q & = & R_{on} T_{on} \\
    R & = & \left (\frac{C + R_L}{2} \right ) \left (\frac{T_{on} + D + \tau}
    {T_{on} + T_{off}} \right ) + C \left (\frac{T_{off} - D - \tau}
    {T_{on} + T_{off}} \right ) \\
    R_L & = & C - \frac{R_{on}(T_{on} + D)}{\eta}
  \end{IEEEeqnarray*}

\subsection{Case 40}
  Conditions:
  \begin{IEEEeqnarray*}{rCl}
    RTT & \ge & T_{on} \\
    RTT & < & T_{on} + T_{off} \\
    RTT & \ge & T_{off} - D \\
    RTT & < & T_{off} + T_{on} - D - \tau
  \end{IEEEeqnarray*}
  Equations:
  \begin{IEEEeqnarray*}{rCl}
    Q & = & \frac{(R_{M1} - 2C + R_L + 2R_{on})(RTT + D - T_{off})}{2} +
    \frac{(R_L - C + 2R_{on})\tau}{2} \\
    && + R_{on}(T_{off} + T_{on} - RTT - D - \tau) \\
    R & = & \left (\frac{C + R_L}{2} \right ) \left (\frac{T_{on} + D + \tau}
    {T_{on} + T_{off}} \right ) + C \left (\frac{T_{off} - D - \tau}
    {T_{on} + T_{off}} \right ) \\
    R_{M1} & = & C + \frac{R_{on}(RTT - T_{off} - T_{on})}{\eta} \\
    R_L & = & C - \frac{R_{on}(T_{on} + D)}{\eta}
  \end{IEEEeqnarray*}

\subsection{Case 41}
  Conditions:
  \begin{IEEEeqnarray*}{rCl}
    RTT & \ge & T_{on} \\
    RTT & < & T_{on} + T_{off} \\
    RTT & \ge & T_{on} + T_{off} - \eta \\
    RTT & < & 2T_{on} + T_{off} - \eta \\
    RTT & \ge & T_{off} - D \\
    RTT & < & T_{off} + T_{on} - D - \tau
  \end{IEEEeqnarray*}
  Equations:
  \begin{IEEEeqnarray*}{rCl}
    Q & = & \frac{(RTT + \eta - T_{on} - T_{off})(R_{M1} - C + R_{on})}{2} + 
    \frac{\tau R_{on}}{2} + R_{on} (T_{off} + T_{on} - RTT - D - \tau) \\
    R & = & C - R_{avg}\frac{2T_{on} + 2D + \tau - \eta}{2T_{on}} \\
    R_{M1} & = & C + \frac{R_{on}(RTT - T_{off} - T_{on})}{\eta}
  \end{IEEEeqnarray*}
